Bank_Proofs.v
@@ -4,6 +4,12 @@ Require Import
   Verdi.Verdi
   Verdi.HandlerMonad.
 
+Require Import
+  Coq.FSets.FMapFacts
+  Coq.Structures.OrderedTypeEx.
+
+Module NatDictWF := WFacts_fun Nat_as_OT NatDict.
+
 Set Bullet Behavior "Strict Subproofs".
 
 Section Bank_Proof.
@@ -12,21 +18,25 @@ Section Bank_Proof.
    * Tactics
    *******)
 
-  (* Repeated unfolding of all handler monads *)
-  Ltac bank_handlers_unfold :=
-    repeat (monad_unfold
-           ; unfold InitState,
+  Ltac simplify_bank_handlers :=
+    repeat ( monad_unfold
+           ; unfold step_async_init, InitState,
                     NetHandler,
                     AgentNetHandler, ServerNetHandler,
                     IOHandler,
-                    AgentIOHandler, ServerIOHandler in *).
+                    AgentIOHandler, ServerIOHandler in *
+           ; simpl in *
+           ; repeat break_match)
+    ; repeat (prove_eq ; clean)
+    ; subst_max
+    ; simpl in *.
 
   (*******
    * Basic lemmas on steps and traces
    *******)
 
-  (* Empty trace => No change in network.
-   * [Converse cannot be proved] *)
+  (* [SAFETY]
+   * Empty trace => No change in network. [Converse cannot be proved] *)
   Lemma step_star_no_trace_no_step :
     forall net net' trace,
       step_async_star net net' trace ->
@@ -40,12 +50,12 @@ Section Bank_Proof.
       - invc H1 ; invc H5.
   Qed.
 
-  (* In a well-formed trace,
-   * every node must be present in Nodes. *)
+  (* [SAFETY]
+   * In a well-formed trace, every node must be present in Nodes. *)
   Lemma trace_well_formed :
     forall net trace trace' n io,
       step_async_star step_async_init net trace ->
-      (trace = [] \/ (trace = trace' ++ [(n, io)] -> (List.In n Nodes))).
+      (trace = [] \/ (trace = trace' ++ [(n, io)] -> (In n Nodes))).
   Proof using.
     intros. invcs H.
     (* net = net' *)
@@ -54,129 +64,149 @@ Section Bank_Proof.
     - right. intuition. apply all_Names_Nodes.
   Qed.
 
-  Definition trace_values (trace : list (name * (input + list output)))
-                          : list Value :=
+  (********
+   * More complex properties
+   ********)
+
+  (* [SAFETY]
+   * Min Value Balance : Over all traces, the returned account value
+   *                     is always greater than the minimum value.
+   *)
+  Inductive min_value_invariant_state : ServerState -> Prop :=
+  | min_value_invariant_nil_state :
+      min_value_invariant_state (NatDict.empty Value)
+  | min_value_invariant_add_state :
+      forall st acc val,
+        min_value_invariant_state st ->
+        val >= minValue ->
+        min_value_invariant_state (NatDict.add acc val st).
+
+  Lemma min_value_invariant_state_values :
+    forall st k v,
+      min_value_invariant_state st ->
+      NatDict.find k st = Some v ->
+      v >= minValue.
+  Proof using.
+    intros. induction H.
+    - apply NatDictWF.find_mapsto_iff, NatDictWF.empty_mapsto_iff in H0.
+      intuition.
+    - apply NatDictWF.find_mapsto_iff, NatDictWF.add_mapsto_iff in H0.
+      intuition. apply NatDictWF.find_mapsto_iff in H3. intuition.
+  Qed.
+
+  Lemma min_value_invariant_server_resp :
+    forall msg st outs st' msgs,
+      min_value_invariant_state st ->
+      ServerNetHandler msg st = (tt, outs, st', msgs) ->
+      (min_value_invariant_state st' /\
+        (forall d a c v,
+          In (d, (netM c (resp (PassMsg a v)))) msgs ->
+          v >= minValue)).
+  Proof using.
+    intros. split ; intros.
+    (* state_values_gt_min_value st' *)
+    - simplify_bank_handlers ; repeat find_inversion ; intuition.
+      (* create *)
+      + apply (min_value_invariant_add_state st a minValue) ; intuition.
+      (* deposit *)
+      + pose proof (min_value_invariant_state_values st a v0) as Hv0. intuition.
+        apply (min_value_invariant_add_state st a (v0 + v)) ; intuition.
+      (* withdraw *)
+      + pose proof (min_value_invariant_state_values st a v0) as Hv0. intuition.
+        apply (min_value_invariant_add_state st a (v0 - v)) ; intuition.
+    (* PassMsg *)
+    - simplify_bank_handlers
+    ; repeat find_inversion
+    ; try (destruct H1 ; try find_inversion ; intuition ; try destruct H0).
+      + pose proof (min_value_invariant_state_values st a v1) as Hv1.
+        intuition.
+      + apply (min_value_invariant_state_values st' a v) ; intuition.
+  Qed.
+
+  Definition values_in_trace (trace : list (name * (input + list output)))
+                             : list Value :=
     flat_map (fun n_io => match n_io with
                           | (Server, _)    => nil
                           | (Agent, inl _) => nil
                           | (Agent, inr listO) =>
                               filterMap (fun o => match o with
-                                                  | netO _ Failed => None
                                                   | netO _ (Passed _ v) => Some v
+                                                  | _                   => None
+                                                  end)
+                                        listO
+                 end)
+              trace.
+
+  Lemma min_value_invariant_step :
+    forall st net net' st' trace,
+      (nwState net) Server = server st ->
+      min_value_invariant_state st ->
+      step_async net net' trace ->
+      (nwState net') Server = server st' ->
+      (min_value_invariant_state st' /\
+        (forall v, In v (values_in_trace trace) -> v >= minValue)).
+  Proof using.
+    intros. split.
+    (* state_values_gt_min_value st' *)
+    - invcs H1 ; break_if ; subst_max.
+      (* NetHandler *)
+      + unfold NetHandler in *. break_match.
+        * invcs e.
+        * break_match. invcs H4. invcs H. monad_unfold. 
+          repeat break_let. invcs H4. invcs Heqp0. destruct u.
+          pose proof (min_value_invariant_server_resp (pBody p) st out st' l).
+          intuition.
+      + simplify_bank_handlers ; try (rewrite H in H2 ; invcs H2 ; intuition).
+      (* IOHandler *)
+      + simplify_bank_handlers.
+        * invcs H.
+        * rewrite H in H5. invcs H5. intuition.
+      + simplify_bank_handlers ; try (rewrite H in H2 ; invcs H2 ; intuition).
+    (* forall v, In v (values_in_trace trace) -> v >= minValue *)
+    - intros. invcs H1 ; break_if.
+      (* NetHandler *)
+      + admit.
+      + apply in_nil in H3. destruct H3.
+      (* IOHandler *)
+      + simplify_bank_handlers ; try contradiction.
+      + apply in_nil in H3. destruct H3.
+  Admitted.
+
+  Theorem min_value_invariant :
+    forall net st trace,
+      step_async_star step_async_init net trace ->
+      (nwState net) Server = server st ->
+      (min_value_invariant_state st /\
+        (forall v, In v (values_in_trace trace) -> v >= minValue)).
+  Proof using.
+    intros.
+    unfold values_in_trace in H0. split. admit.
+  Admitted.
+
+  Definition accounts_in_trace (trace : list (name * (input + list output)))
+                               : list Account :=
+    flat_map (fun n_io => match n_io with
+                          | (Server, _)    => nil
+                          | (Agent, inl _) => nil
+                          | (Agent, inr listO) =>
+                              filterMap (fun o => match o with
+                                                  | netO _ (Passed a _) => Some a
+                                                  | _                   => None
                                                   end)
                                         listO
                  end)
               trace.
 
   (* [SAFETY]
-   * No Negative Value : Over all traces, the returned account value
-   *                     is always non-negative.
-   *)
-  Theorem no_negative_value :
+   * For every account in the trace, we must have a CREATE input. *)
+  Theorem every_account_was_created :
     forall net trace,
       step_async_star step_async_init net trace ->
-      forall v, List.In v (trace_values trace) -> v >= 0.
+      forall a, In a (accounts_in_trace trace) ->
+      exists n c, In (n, inl (netI c (Create a))) trace.
   Proof using.
-    intros net trace H_network_step_star v H_v_in_trace.
-    unfold trace_values in H_v_in_trace.
-    apply in_flat_map in H_v_in_trace.
+  (* TODO: Do it. Do it. Do it. *)
   Admitted.
-
-(* 
-  SAFETY for STATES, no need now
-
-  Definition valid_values (m : ServerState) : Prop := 
-    forall acc v,
-      NatDict.find acc m = Some v ->
-      v >= 0.
-
-  Definition bank_correct (sigma : Name -> State) : Prop :=
-    match (sigma Server) with
-    | agent  _      => False
-    | server sstate => valid_values sstate
-    end.
-
-  Lemma bank_correct_init :
-    bank_correct init_handlers.
-  Proof using.
-    simpl. discriminate.
-  Qed.
-  
-  Definition timeout_case (i : NetInput) (out : list NetOutput) (st : State) (st' : State) (ms : list (Name * NetMsg)) :=
-  match st with
-  | server ss => False
-  | agent _ => exists cid, i = netI cid (Timeout) /\ out = [] /\ ms = []
-  end.
-  
-  Definition create_case (i : NetInput) (out : list NetOutput) (st : State) (st' : State) (ms : list (Name * NetMsg)) :=
-  match st with
-  | server ss => False
-  | agent _ => exists a cid, i = netI cid (Create a) /\ out = [] /\ ms = [(Server, netM cid (req (CreateMsg a)))]
-  end.
-  
-  Definition deposit_case (i : NetInput) (out : list NetOutput) (st : State) (st' : State) (ms : list (Name * NetMsg)) :=
-  match st with
-  | server ss => False
-  | agent _ => exists a v cid, i = netI cid (Deposit a v) /\ out = []  /\ ms = [(Server, netM cid (req (DepositMsg a v)))]
-  end.
-  
-  Definition withdraw_case (i : NetInput) (out : list NetOutput) (st : State) (st' : State) (ms : list (Name * NetMsg)) :=
-  match st with
-  | server ss => False
-  | agent _ => exists a v cid, i = netI cid (Withdraw a v) /\ out = [] /\ ms = [(Server, netM cid (req (WithdrawMsg a v)))]
-  end.
-
-  Definition check_case (i : NetInput) (out : list NetOutput) (st : State) (st' : State) (ms : list (Name * NetMsg)) :=
-  match st with
-  | server ss => False
-  | agent _ => exists a cid, i = netI cid (Check a) /\ out = [] /\ ms = [(Server, netM cid (req (CheckMsg a)))]
-  end.
-
-  Ltac handler_unfold :=
-    repeat (monad_unfold; unfold NetHandler,
-                                 IOHandler,
-                                 ServerNetHandler,
-                                 AgentNetHandler,
-                                 AgentIOHandler,
-                                 ServerIOHandler in .
-  
-  Lemma IOHandler_cases:
-  forall name input state netout state' ms,
-    IOHandler name input state = (netout, state', ms) ->
-    (name = Agent /\ (timeout_case input netout state state' ms \/ create_case input netout state state' ms \/ deposit_case input netout state state' ms \/ withdraw_case input netout state state' ms \/ check_case input netout state state' ms)) \/ (netout = [] /\ state = state' /\ ms = []). 
-  Proof.
-  handler_unfold. intros.
-  repeat break_match;
-  repeat tuple_inversion;
-  [left|left|left|left|left|left|left|right|right|right]; 
-  try intuition.
-  - left. unfold timeout_case. repeat eexists.
-  - right. left. unfold create_case. repeat eexists.
-  - right. right. left. unfold deposit_case. repeat eexists.
-  - right. right. right. left. unfold withdraw_case. repeat eexists.
-  - repeat (try right). unfold check_case. repeat eexists.
-Qed.
-
-  Lemma bank_correct_io_handlers :
-    forall name input sigma st' netout ms,
-      IOHandler name input (sigma name) = (netout, st', ms) ->
-      bank_correct sigma ->
-      bank_correct (update name_eq_dec sigma name st').
-  Proof. 
-  Admitted.
-   
-  Lemma bank_correct_net_handlers :
-    forall p sigma st' out ms,
-      NetHandler (pDst p) (pSrc p) (pBody p) (sigma (pDst p)) = (out, st', ms) ->
-      bank_correct sigma ->
-      bank_correct (update name_eq_dec sigma (pDst p) st').
-  Proof.
-  Admitted.
-  
-  Theorem true_in_reachable_bank_correct :
-  true_in_reachable step_async step_async_init (fun net => bank_correct (nwState net)).
-  Proof.
-  Admitted.*)
 
   (* [SAFETY]
    * Trace Correctness : Simulate the trace on an interpreter and prove that
